Rahmem für die CC-Analyse

Launchbury/CoCallAnalysisImpl.thy
@@ -1,25 +1,99 @@
 theory CoCallAnalysisImpl
-imports CoCallFix ArityAnalysisPreImpl "Arity-Nominal" "Nominal-HOLCF" "Env-Nominal" "Env-HOLCF"
+imports CoCallFix  "Arity-Nominal" "Nominal-HOLCF" "Env-Nominal" "Env-HOLCF"
 begin
 
+fun combined_restrict :: "var set \<Rightarrow> (AEnv \<times> CoCalls) \<Rightarrow> (AEnv \<times> CoCalls)"
+  where "combined_restrict S (env, G) = (env f|` S, cc_restr S G)"
 
-term ArityAnalysisPreImpl.Aexp
-term "\<lambda> x y z. CoCallArityAnalysis.ccFix z (ArityAnalysisPreImpl.Aexp x)"
+lemma combined_restrict_eqvt[eqvt]:
+  shows "\<pi> \<bullet> combined_restrict S p = combined_restrict (\<pi> \<bullet> S) (\<pi> \<bullet> p)"
+  by (cases p) auto
 
+lemma combined_restrict_cont:
+  "cont (\<lambda>x. combined_restrict S x)"
+proof-
+  have "cont (\<lambda>(env, G). combined_restrict S (env, G))" by simp
+  thus ?thesis by (metis split_eta)
+qed
+lemmas cont_compose[OF combined_restrict_cont, cont2cont, simp]
+
+lemma combined_restrict_perm:
+  assumes "supp \<pi> \<sharp>* S" and [simp]: "finite S"
+  shows "combined_restrict S (\<pi> \<bullet> p) = combined_restrict S p"
+proof(cases p)
+  fix env :: AEnv and  G :: CoCalls
+  assume "p = (env, G)"
+  moreover 
+  from assms
+  have "env_restr S (\<pi> \<bullet> env) = env_restr S env" by (rule env_restr_perm)
+  moreover
+  from assms
+  have "cc_restr S (\<pi> \<bullet> G) = cc_restr S G" by (rule cc_restr_perm)
+  ultimately
+  show ?thesis by simp
+qed
+  
 nominal_function
-  Aexp :: "exp \<Rightarrow> (Arity \<rightarrow> AEnv)" and ccExp :: "exp \<Rightarrow> (Arity \<rightarrow> CoCalls)" 
+  cccExp :: "exp \<Rightarrow> (Arity \<rightarrow> AEnv \<times> CoCalls)" 
 where
-  "Aexp (GVar b x) = (\<Lambda> n . AE_singleton x \<cdot> (up \<cdot> n))"
-| "Aexp (Lam [x]. e) = (\<Lambda> n . (Aexp e \<cdot> (pred \<cdot> n)  f|` (fv (Lam [x]. e))))"
-| "Aexp (App e x) = (\<Lambda> n . Aexp e  \<cdot> (inc \<cdot> n) \<squnion> (AE_singleton x \<cdot> (up \<cdot> 0)))"
-| "Aexp (Terms.Let as e) = (\<Lambda> n . fst (CoCallArityAnalysis.ccFix  ccExp Aexp as \<cdot> (Aexp e \<cdot> n, cExp e \<cdot> n)) f|` (fv (Terms.Let as e)))"
+  "cccExp (GVar b x) = (\<Lambda> n . (AE_singleton x \<cdot> (up \<cdot> n), \<bottom>))"
+| "cccExp (Lam [x]. e) = (\<Lambda> n . combined_restrict (fv (Lam [x]. e)) (fst (cccExp e\<cdot>(pred\<cdot>n)), \<bottom>))"
+| "cccExp (App e x) = (\<Lambda> n . (fst (cccExp e\<cdot>(inc\<cdot>n)) \<squnion> (AE_singleton x \<cdot> (up \<cdot> 0)), \<bottom>))"
+| "cccExp (Let as e) = (\<Lambda> n . combined_restrict (fv (Let as e)) (CoCallArityAnalysis.ccFix cccExp as \<cdot> (cccExp e \<cdot> n)))"
+proof-
+case goal1
+    show ?case
+    unfolding eqvt_def cccExp_graph_aux_def
+    apply rule
+    apply (perm_simp)
+    apply (simp add: Abs_cfun_eqvt)
+    done
+next
+case goal3 thus ?case by (metis Terms.exp_strong_exhaust)
+next
+case (goal8 x e x' e')
+  from goal8(5)
+  show ?case
+  proof(rule eqvt_lam_case)
+    fix \<pi> :: perm
+    assume *: "supp (-\<pi>) \<sharp>* (fv (Lam [x]. e) :: var set)" 
+    {
+    fix n
+    have "combined_restrict (fv (Lam [x]. e)) (fst (cccExp_sumC (\<pi> \<bullet> e)\<cdot>(pred\<cdot>n)), \<bottom>) = combined_restrict (fv (Lam [x]. e)) (- \<pi> \<bullet> (fst (cccExp_sumC (\<pi> \<bullet> e)\<cdot>(pred\<cdot>n)), \<bottom>))"
+      by (rule combined_restrict_perm[symmetric, OF *]) simp
+    also have "\<dots> = combined_restrict (fv (Lam [x]. e)) (fst (cccExp_sumC e\<cdot>(pred\<cdot>n)), \<bottom>)"
+      by (simp add: eqvt_at_apply[OF goal8(1)] pemute_minus_self)
+    also note calculation
+    }
+    thus "(\<Lambda> n. combined_restrict (fv (Lam [x]. e)) (fst (cccExp_sumC (\<pi> \<bullet> e)\<cdot>(pred\<cdot>n)), \<bottom>)) = (\<Lambda> n. combined_restrict (fv (Lam [x]. e)) (fst (cccExp_sumC e\<cdot>(pred\<cdot>n)), \<bottom>))" by simp
+  qed
+next
+case (goal13 as body as' body')
+  from goal13(9)
+  show ?case
+  proof (rule eqvt_let_case)
+    fix \<pi> :: perm
+    assume *: "supp (-\<pi>) \<sharp>* (fv (Terms.Let as body) :: var set)"
+    
+    { fix n
+      have "combined_restrict (fv (Terms.Let as body)) (CoCallArityAnalysis.ccFix cccExp_sumC (\<pi> \<bullet> as)\<cdot>(cccExp_sumC (\<pi> \<bullet> body)\<cdot>n))
+      =  combined_restrict (fv (Terms.Let as body)) (- \<pi> \<bullet> (CoCallArityAnalysis.ccFix cccExp_sumC (\<pi> \<bullet> as)\<cdot>(cccExp_sumC (\<pi> \<bullet> body)\<cdot>n)))"
+        by (rule combined_restrict_perm[OF *, symmetric]) simp
+      also have "- \<pi> \<bullet> (CoCallArityAnalysis.ccFix cccExp_sumC (\<pi> \<bullet> as)\<cdot>(cccExp_sumC (\<pi> \<bullet> body)\<cdot>n)) = 
+                       CoCallArityAnalysis.ccFix (- \<pi> \<bullet> cccExp_sumC) as\<cdot>((- \<pi> \<bullet> cccExp_sumC) body\<cdot>n)"
+        by (simp add: pemute_minus_self)
+      also have "CoCallArityAnalysis.ccFix (- \<pi> \<bullet> cccExp_sumC) as = CoCallArityAnalysis.ccFix cccExp_sumC as"
+        by (rule ccFix_cong[OF eqvt_at_apply[OF goal13(1)] refl])
+      also have "(- \<pi> \<bullet> cccExp_sumC) body = cccExp_sumC body"
+        by (rule eqvt_at_apply[OF goal13(2)])
+      also note calculation
+    }
+    thus "(\<Lambda> n. combined_restrict (fv (Terms.Let as body)) (CoCallArityAnalysis.ccFix cccExp_sumC (\<pi> \<bullet> as)\<cdot>(cccExp_sumC (\<pi> \<bullet> body)\<cdot>n))) =
+         (\<Lambda> n. combined_restrict (fv (Terms.Let as body)) (CoCallArityAnalysis.ccFix cccExp_sumC as\<cdot>(cccExp_sumC body\<cdot>n)))" by (simp only:)
+  qed
+qed auto
 
-| "ccExp (GVar b x) = (\<Lambda> n . \<bottom>)"
-| "ccExp (Lam [x]. e) = (\<Lambda> n . \<bottom>)"
-| "ccExp (App e x) = (\<Lambda> n . \<bottom>)"
-| "ccExp (Terms.Let as e) = (\<Lambda> n . \<bottom>)"
-
-
+nominal_termination (eqvt) by lexicographic_order
 
 end
 
